CP in fixing build

theories/L6_PCPS/closure_conversion_invariants.v
@@ -2,7 +2,7 @@
  * Author: Zoe Paraskevopoulou, 2016
  *)
 
-Require Import L6.tactics L6.closure_conversion L6.closure_conversion_util.
+Require Import L6.tactics L6.closure_conversion L6.closure_conversion_util L6.algebra.
 From CertiCoq Require Import cps size_cps cps_util set_util hoisting identifiers ctx
                        Ensembles_util List_util functions eval logical_relations_cc.
 Require Import compcert.lib.Coqlib.
@@ -52,10 +52,12 @@ Section Closure_conversion_invariants.
   Variable pr : prims.
   Variable cenv : ctor_env.
   Variable clo_tag : ctor_tag.
+  
+  Context {fuel : Type} {Hfuel : @fuel_resource fuel} {trace : Type} {Htrace : @trace_resource trace}.
 
   (* Parameterize over the postconditions *)
-  Context (boundL : nat -> PostT)
-          (boundG : PostGT).
+  Context (boundL : nat -> @PostT fuel trace)
+          (boundG : @PostGT fuel trace).
   
   (** ** Semantics preservation proof *)
 
@@ -84,7 +86,7 @@ Section Closure_conversion_invariants.
                       cc_approx_val cenv clo_tag k boundG v v') FVs vs.
   
   (** Invariant about the functions in the current function definition *)
-  Definition Fun_inv k (rho rho' : env) Scope Funs σ genv : Prop :=
+  Definition Fun_inv k (rho rho' : env) Scope Funs genv : Prop :=
     forall f v,
       ~ In _ Scope f ->
       In var Funs f ->
@@ -92,21 +94,21 @@ Section Closure_conversion_invariants.
       exists env rho1 B1 f1 rho2 B2 f2,
         M.get (genv f) rho' = Some env /\
         v = (Vfun rho1 B1 f1) /\
-        ~ In _ Scope (σ f) /\
-        M.get (σ f) rho' = Some (Vfun rho2 B2 f2) /\
+        ~ In _ Scope f /\
+        M.get f rho' = Some (Vfun rho2 B2 f2) /\
         cc_approx_val cenv clo_tag k boundG
                       (Vfun rho1 B1 f1)
                       (Vconstr clo_tag [(Vfun rho2 B2 f2) ; env]).
 
   (** Invariant about the functions in the current function definition *)
-  Definition GFun_inv k (rho rho' : env) Scope GFuns σ : Prop :=
+  Definition GFun_inv k (rho rho' : env) Scope GFuns : Prop :=
     forall f v c,
       In var GFuns f ->
       M.get f rho = Some v  ->
       exists rho1 B1 f1 rho2 B2 f2,
         v = (Vfun rho1 B1 f1) /\
-        ~ In _ Scope (σ f) /\ (* Check if needed *)
-        M.get (σ f) rho' = Some (Vfun rho2 B2 f2) /\
+        ~ In _ Scope f /\ (* Check if needed *)
+        M.get f rho' = Some (Vfun rho2 B2 f2) /\
         cc_approx_val cenv clo_tag k boundG
                       (Vfun rho1 B1 f1)
                       (Vconstr clo_tag [(Vfun rho2 B2 f2) ; (Vconstr c [])]).
@@ -115,10 +117,10 @@ Section Closure_conversion_invariants.
   (** * Lemmas about Fun_inv *)
 
   (** Extend the first environment with a variable in not in [Funs] *)
-  Lemma Fun_inv_monotonic k m rho1 rho2 Scope Funs σ Γ :
-    Fun_inv k rho1 rho2 Scope Funs σ Γ ->
+  Lemma Fun_inv_monotonic k m rho1 rho2 Scope Funs Γ :
+    Fun_inv k rho1 rho2 Scope Funs Γ ->
     m <= k ->
-    Fun_inv m rho1 rho2 Scope Funs σ Γ.
+    Fun_inv m rho1 rho2 Scope Funs Γ.
   Proof.
     intros Hinv Hin f v' Hninf Hinf Hget.
     edestruct Hinv with (f := f) as
@@ -129,23 +131,21 @@ Section Closure_conversion_invariants.
 
   (** Extend the two environments with a variable that is not the current environment
     argument (i.e. [Γ]) *)
-  Lemma Fun_inv_set k rho rho' Scope Funs σ genv f rho1 B1 f1 rho2 B2 f2 env:
-    Fun_inv k rho rho' Scope Funs σ genv ->
+  Lemma Fun_inv_set k rho rho' Scope Funs genv f rho1 B1 f1 rho2 B2 f2 env:
+    Fun_inv k rho rho' Scope Funs genv ->
     
-    ~ In _ (image genv (Funs \\ Scope)) (σ f) ->
-    σ f <> genv f ->
+    ~ In _ (image genv (Funs \\ Scope)) f ->
+    f <> genv f ->
 
-    ~ In _ Scope (σ f) ->
-    ~ In _ (image σ (Funs \\ Scope)) (σ f) ->
-
+    
     M.get (genv f) rho' = Some env ->
     (cc_approx_val cenv clo_tag k boundG (Vfun rho1 B1 f1)
                    (Vconstr clo_tag [(Vfun rho2 B2 f2) ; env])) ->
     Fun_inv k (M.set f (Vfun rho1 B1 f1) rho)
-            (M.set (σ f) (Vfun rho2 B2 f2) rho')
-            Scope (Union _ (Singleton _ f) Funs) σ genv.
+            (M.set f (Vfun rho2 B2 f2) rho')
+            Scope (Union _ (Singleton _ f) Funs) genv.
   Proof.
-    intros Hinv Hneq Hnin Hnin' Hnin'' Hget Hv f'' v Hnin''' Hin Hget'.
+    intros Hinv Hneq Hnin Hget Hv f'' v Hnin''' Hin Hget'.
     destruct (peq f'' f); subst.
     - repeat eexists; eauto. rewrite M.gso; eauto.
       now rewrite M.gss in Hget'; inv Hget'; eauto.
@@ -157,8 +157,7 @@ Section Closure_conversion_invariants.
       repeat eexists; eauto. rewrite M.gso. eassumption. 
       intros Hc. eapply Hneq. rewrite <- Hc. eapply In_image. constructor; eauto.
       rewrite M.gso. now eauto.
-      intros Hc. eapply Hnin''. eexists; eauto. split; [| eassumption ].
-      now constructor; eauto.
+      intros Hc. subst. contradiction.
   Qed.
 
   (* (** Rename the environment parameter *) *)
@@ -178,25 +177,21 @@ Section Closure_conversion_invariants.
   (* Qed. *)
   
   (** Extend [Scope] with a set that does not shadow the new function names *)
-  Lemma Fun_inv_mon k rho1 rho2 Scope Scope' Funs σ genv :
-    Disjoint _ (image σ (Funs \\ Scope)) Scope' ->
-    Fun_inv k rho1 rho2 Scope Funs σ genv ->
-    Fun_inv k rho1 rho2 (Union _ Scope' Scope) Funs σ genv.
+  Lemma Fun_inv_mon k rho1 rho2 Scope Scope' Funs genv :
+    Fun_inv k rho1 rho2 Scope Funs genv ->
+    Fun_inv k rho1 rho2 (Union _ Scope' Scope) Funs genv.
   Proof.
-    intros Hd Hinv f v Hninf Hinf Hget.
+    intros (* Hd *) Hinv f v Hninf Hinf Hget.
     edestruct Hinv with (f := f) as
         [vs' [rho3 [B3 [f3 [rho4 [B4 [f4 [Hget1 [Heq2 [Ηnin2 [Hget2 Happrox]]]]]]]]]]]; eauto.
     repeat eexists; eauto.
-    intros Hc; inv Hc. eapply Hd. constructor; eauto. 
-    eexists; eauto. split; [| now eauto ]. now constructor; eauto.
-    now eauto.
   Qed.
 
   (** Extend the first environment with a variable in [Scope] *)
-  Lemma Fun_inv_set_In_Scope_l k rho1 rho2 Scope Funs σ Γ x v :
+  Lemma Fun_inv_set_In_Scope_l k rho1 rho2 Scope Funs Γ x v :
     In _ Scope x ->
-    Fun_inv k rho1 rho2 Scope Funs σ Γ ->
-    Fun_inv k (M.set x v rho1) rho2 Scope Funs σ Γ.
+    Fun_inv k rho1 rho2 Scope Funs Γ ->
+    Fun_inv k (M.set x v rho1) rho2 Scope Funs Γ.
   Proof.
     intros Hin Hinv f v' Hninf Hinf Hget.
     eapply Hinv; eauto. rewrite M.gso in Hget.
@@ -204,10 +199,10 @@ Section Closure_conversion_invariants.
   Qed.
 
     (** Extend the first environment with a variable in not in [Funs] *)
-  Lemma Fun_inv_set_not_In_Funs_l k rho1 rho2 Scope Funs σ Γ x v :
+  Lemma Fun_inv_set_not_In_Funs_l k rho1 rho2 Scope Funs Γ x v :
     ~ In _ Funs x  ->
-    Fun_inv k rho1 rho2 Scope Funs σ Γ ->
-    Fun_inv k (M.set x v rho1) rho2 Scope Funs σ Γ.
+    Fun_inv k rho1 rho2 Scope Funs Γ ->
+    Fun_inv k (M.set x v rho1) rho2 Scope Funs Γ.
   Proof.
     intros Hin Hinv f v' Hninf Hinf Hget.
     eapply Hinv; eauto. rewrite M.gso in Hget.
@@ -215,10 +210,10 @@ Section Closure_conversion_invariants.
   Qed.
 
   (** Extend the first environment with a variable in not in [Funs] *)
-  Lemma Fun_inv_funs_monotonic k rho1 rho2 Scope Funs Funs' σ Γ :
-    Fun_inv k rho1 rho2 Scope Funs σ Γ ->
+  Lemma Fun_inv_funs_monotonic k rho1 rho2 Scope Funs Funs' Γ :
+    Fun_inv k rho1 rho2 Scope Funs Γ ->
     Funs' \subset Funs -> 
-    Fun_inv k rho1 rho2 Scope Funs' σ Γ.
+    Fun_inv k rho1 rho2 Scope Funs' Γ.
   Proof.
     intros Hin Hinv f v' Hninf Hinf Hget.
     eapply Hin; eauto.
@@ -226,11 +221,11 @@ Section Closure_conversion_invariants.
 
   (** Extend the second environment with a variable in [Scope] that is different
     from [Γ] *)
-  Lemma Fun_inv_set_In_Scope_r_not_Γ k rho1 rho2 Scope Funs σ Γ x v :
+  Lemma Fun_inv_set_In_Scope_r_not_Γ k rho1 rho2 Scope Funs Γ x v :
     In _ Scope x ->
     ~ In _ (image Γ (Funs \\ Scope)) x ->
-    Fun_inv k rho1 rho2 Scope Funs σ Γ ->
-    Fun_inv k rho1 (M.set x v rho2) Scope Funs σ Γ.
+    Fun_inv k rho1 rho2 Scope Funs Γ ->
+    Fun_inv k rho1 (M.set x v rho2) Scope Funs Γ.
   Proof.
     intros Hin Hnin Hinv f v1 Hninf Hinf Hget.
     edestruct Hinv with (f := f) as
@@ -244,11 +239,11 @@ Section Closure_conversion_invariants.
 
   (** Extend the second environment with a variable not in [Funs] that is different
     from Γ *)
-  Lemma Fun_inv_set_not_In_Funs_r_not_Γ k rho1 rho2 Scope Funs σ Γ x v :
-    ~ In _ (image σ (Setminus _ Funs Scope)) x ->
+  Lemma Fun_inv_set_not_In_Funs_r_not_Γ k rho1 rho2 Scope Funs Γ x v :
+    ~ In _ (Funs \\ Scope) x ->
     ~ In _ (image Γ (Funs \\ Scope)) x ->
-    Fun_inv k rho1 rho2 Scope Funs σ Γ ->
-    Fun_inv k rho1 (M.set x v rho2) Scope Funs σ Γ.
+    Fun_inv k rho1 rho2 Scope Funs Γ ->
+    Fun_inv k rho1 (M.set x v rho2) Scope Funs Γ.
   Proof.
     intros Hnin Hneq Hinv f v1 Hninf Hinf Hget.
     edestruct Hinv with (f := f) as
@@ -258,16 +253,15 @@ Section Closure_conversion_invariants.
     intros Hc. subst. eapply Hneq. eapply In_image. constructor; eauto.
 
     rewrite M.gso. now eauto.
-    intros Hc. subst. eapply Hnin.
-    now eexists; eauto.
+    intros Hc. subst. eapply Hnin. constructor; eauto.  
   Qed.
 
   (** Extend the first environment with a list of variables in [Scope] *)
-  Lemma Fun_inv_set_lists_In_Scope_l k rho1 rho1' rho2 Scope Funs σ Γ xs vs :
+  Lemma Fun_inv_set_lists_In_Scope_l k rho1 rho1' rho2 Scope Funs Γ xs vs :
     Included _ (FromList xs) Scope ->
-    Fun_inv k rho1 rho2 Scope Funs σ Γ ->
+    Fun_inv k rho1 rho2 Scope Funs Γ ->
     set_lists xs vs rho1 = Some rho1' ->
-    Fun_inv k rho1' rho2 Scope Funs σ Γ.
+    Fun_inv k rho1' rho2 Scope Funs Γ.
   Proof.
     revert rho1 rho1' vs. induction xs; intros rho1 rho1' vs.
     - intros Hinc Hfun Hset. inv Hset.
@@ -287,12 +281,12 @@ Section Closure_conversion_invariants.
 
 
   (** Extend the second environment with a variable in [Scope] *)
-  Lemma Fun_inv_set_In_Scope_r k rho1 rho2 Scope Funs σ Γ x v v' B :
+  Lemma Fun_inv_set_In_Scope_r k rho1 rho2 Scope Funs Γ x v v' B :
     In _ Scope x ->
-    ~ In _ (image σ (Setminus _ Funs Scope)) x ->
+    ~ In _ (Funs \\ Scope) x ->
     Funs \subset name_in_fundefs B ->
-    Fun_inv k rho1 (M.set Γ v rho2) Scope Funs σ (extend_fundefs' id B Γ) ->
-    Fun_inv k rho1 (M.set Γ v (M.set x v' rho2)) Scope Funs σ (extend_fundefs' id B Γ).
+    Fun_inv k rho1 (M.set Γ v rho2) Scope Funs (extend_fundefs' id B Γ) ->
+    Fun_inv k rho1 (M.set Γ v (M.set x v' rho2)) Scope Funs (extend_fundefs' id B Γ).
   Proof.
     intros Hin Hnin Hsub Hinv f v1 Hninf Hinf Hget.
     edestruct Hinv with (f := f) as
@@ -301,24 +295,23 @@ Section Closure_conversion_invariants.
     rewrite M.gss in Hget1; inv Hget1. 
     repeat eexists; eauto.
     rewrite extend_fundefs'_get_s, M.gss. reflexivity. now eauto.
-    destruct_with_eqn (peq (σ f) Γ).
+    destruct_with_eqn (peq f Γ).
     - subst. now rewrite M.gss in *.
     - rewrite M.gso; eauto. rewrite M.gso in Hget2; eauto.
       rewrite M.gso; eauto.
       intros Hc; subst. eapply Hnin. eexists; eauto.
-      split; [| now eauto]. constructor; eauto.
     - eauto.
   Qed.
 
   
   (** Extend the second environment with a list of variables in [Scope] *)
-  Lemma Fun_inv_set_lists_In_Scope_r k rho1 rho2 rho2' Scope Funs σ Γ xs vs v B :
+  Lemma Fun_inv_set_lists_In_Scope_r k rho1 rho2 rho2' Scope Funs Γ xs vs v B :
     Included _ (FromList xs) Scope ->
-    Disjoint _ (image σ (Setminus _ Funs Scope)) (FromList xs) ->
+    Disjoint _ (Funs \\ Scope) (FromList xs) ->
     Funs \subset name_in_fundefs B ->
-    Fun_inv k rho1 (M.set Γ v rho2) Scope Funs σ (extend_fundefs' id B Γ) ->
+    Fun_inv k rho1 (M.set Γ v rho2) Scope Funs (extend_fundefs' id B Γ) ->
     set_lists xs vs rho2 = Some rho2' ->
-    Fun_inv k rho1 (M.set Γ v rho2') Scope Funs σ (extend_fundefs' id B Γ).
+    Fun_inv k rho1 (M.set Γ v rho2') Scope Funs (extend_fundefs' id B Γ).
   Proof.
     revert rho2 rho2' vs. induction xs; intros rho2 rho2' vs.
     - intros Hinc Hd Hsub Hfun Hset. inv Hset.
@@ -341,12 +334,12 @@ Section Closure_conversion_invariants.
   Qed.
 
   (** Redefine the environment argument in the second environment *)
-  Lemma Fun_inv_reset k rho rho' B B' v Scope Funs σ Γ :
+  Lemma Fun_inv_reset k rho rho' B B' v Scope Funs Γ :
     ~ In _ (name_in_fundefs B) Γ ->
     Funs \subset name_in_fundefs B' ->
     M.get Γ rho' = Some v ->
-    Fun_inv k rho (def_funs B B rho' rho') Scope Funs σ (extend_fundefs' id B' Γ) ->
-    Fun_inv k rho (M.set Γ v (def_funs B B rho' rho')) Scope Funs σ (extend_fundefs' id B' Γ).
+    Fun_inv k rho (def_funs B B rho' rho') Scope Funs (extend_fundefs' id B' Γ) ->
+    Fun_inv k rho (M.set Γ v (def_funs B B rho' rho')) Scope Funs (extend_fundefs' id B' Γ).
   Proof. 
     intros Hnin Hsub Hget Hinv f v1 Hninf Hinf Hget'.
     edestruct Hinv with (f := f) as
@@ -357,7 +350,7 @@ Section Closure_conversion_invariants.
     repeat eexists.    
     - now rewrite M.gss.
     - eauto.
-    - destruct (peq (σ f) Γ); subst.
+    - destruct (peq f Γ); subst.
       rewrite def_funs_neq in Hget2; eauto.  subst_exp.
       rewrite M.gss. reflexivity.
 
@@ -370,7 +363,7 @@ Section Closure_conversion_invariants.
 
   Global Instance Fun_inv_proper :
     Proper (Logic.eq ==> Logic.eq ==> Logic.eq ==> Same_set var ==>
-                     Logic.eq ==> Logic.eq ==> Logic.eq ==> iff)
+                     Logic.eq ==> Logic.eq ==> iff)
            (Fun_inv).
   Proof.
     constructor; intros Hinv; subst;
@@ -382,19 +375,14 @@ Section Closure_conversion_invariants.
   
   (** Define a block of functions in the first environment and put them in the
     current scope *)
-  Lemma Fun_inv_def_funs_l k rho rho' B1 B1' Scope Funs σ Γ:
-    Disjoint _ (image σ (Setminus _ Funs Scope)) (name_in_fundefs B1') -> 
-    Fun_inv k rho rho' Scope Funs σ Γ ->
-    Fun_inv k (def_funs B1 B1' rho rho) rho'
-            (Union _ (name_in_fundefs B1')  Scope) Funs σ Γ.
+  Lemma Fun_inv_def_funs_l k rho rho' B1 B1' Scope Funs Γ:
+    Fun_inv k rho rho' Scope Funs Γ ->
+    Fun_inv k (def_funs B1 B1' rho rho) rho' (Union _ (name_in_fundefs B1')  Scope) Funs Γ.
   Proof.
-    intros HD Hinv f v1 Hninf Hinf Hget. rewrite def_funs_neq in Hget; eauto.
+    intros Hinv f v1 Hninf Hinf Hget. rewrite def_funs_neq in Hget; eauto.
     edestruct Hinv with (f := f) as
         [vs' [rho3 [B3 [f3 [rho4 [B4 [f4 [Hget1 [Heq2 [Ηnin2 [Hget2 Happrox]]]]]]]]]]]; eauto.
     subst. repeat eexists; eauto.
-    intros Hc; inv Hc; eauto.
-    eapply HD. econstructor; eauto.
-    eexists; split; [| now eauto ]. constructor; eauto.
   Qed.
 
 
@@ -409,39 +397,30 @@ Section Closure_conversion_invariants.
 
   (** Define a block of functions in the second environment and put the in the
     current scope *)
-  Lemma Fun_inv_def_funs_r k rho rho' B1 B1' Scope Funs σ genv :
+  Lemma Fun_inv_def_funs_r k rho rho' B1 B1' Scope Funs genv :
     Disjoint _ (name_in_fundefs B1') (image genv (Funs \\ Scope)) ->
-    Disjoint _ (image σ (Setminus _ Funs Scope)) (name_in_fundefs B1') -> 
-    Fun_inv k rho rho' Scope Funs σ genv ->
-    Fun_inv k rho (def_funs B1 B1' rho' rho')
-            ((name_in_fundefs B1') :|: Scope) Funs σ genv.
+    Fun_inv k rho rho' Scope Funs genv ->
+    Fun_inv k rho (def_funs B1 B1' rho' rho') ((name_in_fundefs B1') :|: Scope) Funs genv.
   Proof.
-    intros Hnin HD Hinv f v1 Hninf Hinf Hget.
+    intros Hnin Hinv f v1 Hninf Hinf Hget.
     edestruct Hinv with (f := f) as
         [vs' [rho3 [B3 [f3 [rho4 [B4 [f4 [Hget1 [Heq2 [Ηnin2 [Hget2 Happrox]]]]]]]]]]]; eauto.
     subst. repeat eexists; eauto.
     rewrite def_funs_neq; eauto. simpl. eapply Disjoint_In_l. eapply Disjoint_sym. eassumption.
     eapply In_image. constructor; eauto.
-    
-    intros Hc; inv Hc; eauto. 
-    eapply HD. econstructor; eauto. eexists;  split; [| now eauto ].
-    now constructor; eauto.
     rewrite def_funs_neq; eauto. 
-    intros Hc. eapply HD. constructor; eauto. eexists; split; [| now eauto ].
-    now constructor; eauto.
   Qed.
 
   (** Define a block of functions in both environments and put the in the
     current scope *)
-  Lemma Fun_inv_def_funs k rho rho' B1 B1' B2 B2' Scope Funs σ genv:
+  Lemma Fun_inv_def_funs k rho rho' B1 B1' B2 B2' Scope Funs genv:
     Disjoint _ (name_in_fundefs B2') (image genv (Funs \\ Scope)) ->
-    Disjoint _ (image σ (Setminus _ Funs Scope)) (name_in_fundefs B1') ->
-    Disjoint _ (image σ (Setminus _ Funs Scope)) (name_in_fundefs B2') ->
-    Fun_inv k rho rho' Scope Funs σ genv ->
+    Disjoint _ (Funs \\ Scope) (name_in_fundefs B2') ->
+    Fun_inv k rho rho' Scope Funs genv ->
     Fun_inv k  (def_funs B1 B1' rho rho) (def_funs B2 B2' rho' rho')
-            Scope (Funs \\ (name_in_fundefs B1')) σ genv.
+            Scope (Funs \\ (name_in_fundefs B1')) genv.
   Proof.
-    intros Hnin2 HD1 HD2 Hinv f v1 Hninf Hinf Hget. inv Hinf.
+    intros Hnin2 HD1 (*  HD2 *) Hinv f v1 Hninf Hinf Hget. inv Hinf.
     rewrite def_funs_neq in Hget; eauto.
     edestruct Hinv with (f := f) as
         [vs' [rho3 [B3 [f3 [rho4 [B4 [f4 [Hget1 [Heq2 [Ηnin2 [Hget2 Happrox]]]]]]]]]]]; eauto.
@@ -450,8 +429,7 @@ Section Closure_conversion_invariants.
     rewrite def_funs_neq; eauto. eapply Disjoint_In_l. eapply Disjoint_sym. eassumption.
     eapply In_image. constructor; eauto.
     rewrite def_funs_neq; eauto.
-    intros Hc. eapply HD2. econstructor; eauto. eexists; split; [| now eauto ].
-    now constructor; eauto.
+    intros Hc. eapply HD1. econstructor; eauto. econstructor; eauto.
   Qed.
   
   (** * Lemmas about FV_inv *)
@@ -511,8 +489,6 @@ Section Closure_conversion_invariants.
     intros [c' [g [Hget [Hc HInv]]]]. do 2 eexists; split; eauto.
     split; eauto.
     eapply Forall2_monotonic_strong; [| eassumption ]; eauto.
-    intros; eauto. eapply H1; eauto.
-    intros Hc'; eapply H4. constructor; eauto.  
   Qed.
 
   Lemma FV_inv_monotonic k j rho rho' Scope GFuns Funs c Γ FVs :
@@ -610,32 +586,29 @@ Section Closure_conversion_invariants.
 
   (** Extend the two environments with a variable that is not the current environment
     argument (i.e. [Γ]) *)
-  Lemma GFun_inv_set k rho rho' Scope GFuns σ f rho1 B1 f1 rho2 B2 f2:
-    GFun_inv k rho rho' Scope GFuns σ ->
-    ~ In _ Scope (σ f) ->
-    ~ In _ (image σ (GFuns \\ [set f])) (σ f) ->
+  Lemma GFun_inv_set k rho rho' Scope GFuns f rho1 B1 f1 rho2 B2 f2:
+    GFun_inv k rho rho' Scope GFuns ->
+    ~ In _ Scope f ->
     (forall c, f \in GFuns ->
           cc_approx_val cenv clo_tag k boundG (Vfun rho1 B1 f1) (Vconstr clo_tag [(Vfun rho2 B2 f2) ; Vconstr c []])) ->
-    GFun_inv k (M.set f (Vfun rho1 B1 f1) rho) (M.set (σ f) (Vfun rho2 B2 f2) rho') Scope GFuns σ.
+    GFun_inv k (M.set f (Vfun rho1 B1 f1) rho) (M.set f (Vfun rho2 B2 f2) rho') Scope GFuns.
   Proof.
-    intros Hinv Hnin Hnin' Hv f'' v Hnin'' Hin Hget'.
+    intros Hinv Hnin (* Hnin' *) Hv f'' v Hnin'' Hin Hget'.
     destruct (peq f'' f); subst; eauto.
     - rewrite M.gss in Hget'. inv Hget'. repeat eexists; eauto.
       now rewrite M.gss.
     - rewrite M.gso in Hget'; eauto.
-      edestruct Hinv with (f0 := f'') as
+      edestruct Hinv with (f := f'') as
           [rho3 [B3 [f3 [rho4 [B4 [f4 [Heq [Ηnin2 [Hget2 Happrox]]]]]]]]]; subst; eauto.
-      constructor; eauto. intros Hc. inv Hc. congruence. repeat eexists; eauto.
-      rewrite M.gso. now eauto. 
-      intros Hc. eapply Hnin'. rewrite <- Hc. eapply In_image. constructor; eauto.
-      intros Hc'. inv Hc'. contradiction.
+      repeat eexists; eauto.
+      rewrite M.gso. now eauto. eassumption.
   Qed.
   
   (** Extend the first environment with a variable not in [GFuns] *)
-  Lemma GFun_inv_set_not_In_GFuns_l k rho1 rho2 Scope GFuns σ x v :
+  Lemma GFun_inv_set_not_In_GFuns_l k rho1 rho2 Scope GFuns x v :
     ~ x \in GFuns ->
-    GFun_inv k rho1 rho2 Scope GFuns σ ->
-    GFun_inv k (M.set x v rho1) rho2 Scope GFuns σ.
+    GFun_inv k rho1 rho2 Scope GFuns ->
+    GFun_inv k (M.set x v rho1) rho2 Scope GFuns.
   Proof.
     intros Hnin Hinv f v' c Hin Hget.
     eapply Hinv; eauto. rewrite M.gso in Hget.
@@ -643,25 +616,25 @@ Section Closure_conversion_invariants.
   Qed.
 
   (** Extend the second environment with a variable in [GFuns] *)
-  Lemma GFun_inv_set_not_In_GFuns_r k rho1 rho2 Scope GFuns σ x v :
-    ~ x \in (image σ GFuns) ->
-    GFun_inv k rho1 rho2 Scope GFuns σ ->
-    GFun_inv k rho1 (M.set x v rho2) Scope GFuns σ.
+  Lemma GFun_inv_set_not_In_GFuns_r k rho1 rho2 Scope GFuns x v :
+    ~ x \in GFuns ->
+    GFun_inv k rho1 rho2 Scope GFuns ->
+    GFun_inv k rho1 (M.set x v rho2) Scope GFuns.
   Proof.
     intros Hnin Hinv f v' c Hin Hget.
     edestruct Hinv as
         [rho3 [B3 [f3 [rho4 [B4 [f4 [Heq2 [Ηnin2 [Hget2 Happrox]]]]]]]]]; eauto.
     repeat eexists; eauto.
     rewrite M.gso. eassumption.
-    intros Hc. eapply Hnin. subst. eapply In_image. eassumption. 
+    intros Hc. eapply Hnin. subst. eassumption.
   Qed.
 
   (** Extend the first environment with a variable not in [GFuns] *)
-  Lemma GFun_inv_setlist_not_In_GFuns_l k rho1 rho1' rho2 Scope GFuns σ xs vs :
+  Lemma GFun_inv_setlist_not_In_GFuns_l k rho1 rho1' rho2 Scope GFuns xs vs :
     Disjoint _ (FromList xs) GFuns ->
     set_lists xs vs rho1 = Some rho1' ->
-    GFun_inv k rho1 rho2 Scope GFuns σ ->
-    GFun_inv k rho1' rho2 Scope GFuns σ.
+    GFun_inv k rho1 rho2 Scope GFuns ->
+    GFun_inv k rho1' rho2 Scope GFuns.
   Proof.
     revert rho1 rho1' vs. induction xs; intros rho1 rho1' vs.
     - intros Hinc Hset Hfun. inv Hset.
@@ -679,11 +652,11 @@ Section Closure_conversion_invariants.
   Qed.
 
   (** Extend the second environment with a list not in [GFuns] *)
-  Lemma GFun_inv_setlist_not_In_GFuns_r k rho1 rho2' rho2 Scope GFuns σ xs vs :
-    Disjoint _ (FromList xs) (image σ GFuns) ->
+  Lemma GFun_inv_setlist_not_In_GFuns_r k rho1 rho2' rho2 Scope GFuns xs vs :
+    Disjoint _ (FromList xs) GFuns ->
     set_lists xs vs rho2 = Some rho2' ->
-    GFun_inv k rho1 rho2 Scope GFuns σ ->
-    GFun_inv k rho1 rho2' Scope GFuns σ.
+    GFun_inv k rho1 rho2 Scope GFuns ->
+    GFun_inv k rho1 rho2' Scope GFuns.
   Proof.
     revert rho2 rho2' vs. induction xs; intros rho2 rho2' vs.
     - intros Hinc Hset Hfun. inv Hset.
@@ -701,36 +674,36 @@ Section Closure_conversion_invariants.
   Qed.
 
   (** Extend the first environment with funs not in [GFuns] *)
-  Lemma GFun_inv_def_funs_not_In_GFuns_l k rho1 rho2 Scope GFuns σ B1 B1' :
+  Lemma GFun_inv_def_funs_not_In_GFuns_l k rho1 rho2 Scope GFuns B1 B1' :
     Disjoint _ (name_in_fundefs B1') GFuns ->
-    GFun_inv k rho1 rho2 Scope GFuns σ ->
-    GFun_inv k (def_funs B1 B1' rho1 rho1) rho2 Scope GFuns σ.
+    GFun_inv k rho1 rho2 Scope GFuns ->
+    GFun_inv k (def_funs B1 B1' rho1 rho1) rho2 Scope GFuns.
   Proof.
     intros HD Hinv f v1 c Hinf Hget. rewrite def_funs_neq in Hget; eauto.
     intros Hc. eapply HD. constructor; eauto.
   Qed.
 
-  Lemma GFun_inv_def_funs_not_In_GFuns_r k rho rho' B1 B1' Scope GFuns σ :
-    Disjoint _ (image σ GFuns) (name_in_fundefs B1') ->
-    GFun_inv k rho rho' Scope GFuns σ ->
-    GFun_inv k rho (def_funs B1 B1' rho' rho') Scope GFuns σ.
+  Lemma GFun_inv_def_funs_not_In_GFuns_r k rho rho' B1 B1' Scope GFuns :
+    Disjoint _ GFuns (name_in_fundefs B1') ->
+    GFun_inv k rho rho' Scope GFuns ->
+    GFun_inv k rho (def_funs B1 B1' rho' rho') Scope GFuns.
   Proof.
     intros HD Hinv f v1 c Hinf Hget. setoid_rewrite def_funs_neq; eauto.
     intros Hc. eapply HD. constructor; sets.
   Qed.
 
-  Lemma GFun_inv_antimon k rho rho' Scope GFuns GFuns' σ :
-     GFun_inv k rho rho' Scope GFuns σ ->
+  Lemma GFun_inv_antimon k rho rho' Scope GFuns GFuns' :
+     GFun_inv k rho rho' Scope GFuns ->
      GFuns' \subset GFuns ->
-     GFun_inv k rho rho' Scope GFuns' σ .
+     GFun_inv k rho rho' Scope GFuns'.
   Proof.
     intros Hg Hsub f v1 Hinf Hget; eauto.
   Qed.
 
-  Lemma GFun_inv_Scope_antimon k rho rho' Scope Scope' GFuns σ :
+  Lemma GFun_inv_Scope_antimon k rho rho' Scope Scope' GFuns :
     Scope' \subset Scope ->               
-    GFun_inv k rho rho' Scope GFuns σ ->
-    GFun_inv k rho rho' Scope' GFuns σ.
+    GFun_inv k rho rho' Scope GFuns ->
+    GFun_inv k rho rho' Scope' GFuns.
   Proof.
     intros Hd Hg f v1 c Hinf Hget; eauto.
     edestruct Hg as (rho1 & B1 & f1 & rho2 & B2 & f2 & Heq1 & Hnin & Hget1 & Hcc); eauto.
@@ -738,22 +711,21 @@ Section Closure_conversion_invariants.
   Qed. 
 
 
-  Lemma GFun_inv_Scope k rho rho' Scope Scope' GFuns σ :
-    Disjoint _ Scope' (image σ GFuns) -> 
-    GFun_inv k rho rho' Scope GFuns σ ->
-    GFun_inv k rho rho' Scope' GFuns σ.
+  Lemma GFun_inv_Scope k rho rho' Scope Scope' GFuns :
+    Disjoint _ Scope' GFuns -> 
+    GFun_inv k rho rho' Scope GFuns ->
+    GFun_inv k rho rho' Scope' GFuns.
   Proof.
     intros Hd Hg f v1 c Hinf Hget; eauto.
     edestruct Hg as (rho1 & B1 & f1 & rho2 & B2 & f2 & Heq1 & Hnin & Hget1 & Hcc); eauto.
     repeat eexists; eauto.
     intros Hc. eapply Hd. constructor; eauto.
-    eapply In_image. eassumption.
   Qed. 
 
-  Lemma GFun_inv_monotonic k j rho rho' Scope GFuns σ :
-    GFun_inv k rho rho' Scope GFuns σ ->
+  Lemma GFun_inv_monotonic k j rho rho' Scope GFuns :
+    GFun_inv k rho rho' Scope GFuns ->
     j <= k ->
-    GFun_inv j rho rho' Scope GFuns σ.
+    GFun_inv j rho rho' Scope GFuns.
   Proof.
     intros Hg Hleq c f v1 Hinf Hget; eauto.
     edestruct Hg as (rho1 & B1 & f1 & rho2 & B2 & f2 & Heq1 & Hnin & Hget1 & Hcc); eauto.
@@ -761,33 +733,31 @@ Section Closure_conversion_invariants.
     eapply cc_approx_val_monotonic; eauto.
   Qed.
   
-  Lemma GFun_inv_Scope_extend k rho rho' Scope Scope' GFuns σ :
-    Disjoint _ (image σ GFuns) Scope' ->
-    GFun_inv k rho rho' Scope GFuns σ ->
-    GFun_inv k rho rho' (Scope' :|: Scope) GFuns σ.
+  Lemma GFun_inv_Scope_extend k rho rho' Scope Scope' GFuns :
+    Disjoint _ GFuns Scope' ->
+    GFun_inv k rho rho' Scope GFuns ->
+    GFun_inv k rho rho' (Scope' :|: Scope) GFuns.
   Proof.
     intros Hdis Hg f v1 c1 Hinf Hget; eauto.
     edestruct Hg as (rho1 & B1 & f1 & rho2 & B2 & f2 & Heq & Hnin & Hget' & Hcc); eauto.
     subst. repeat eexists; eauto.
     intros Hc. inv Hc; eauto.
     eapply Hdis. constructor; eauto.
-    now eapply In_image. 
   Qed.
 
-  Lemma GFun_inv_fuse k rho rho' Scope1 Scope2 GFuns1 GFuns2 σ names FVs { Hd : Decidable names} :
+  Lemma GFun_inv_fuse k rho rho' Scope1 Scope2 GFuns1 GFuns2 names FVs { Hd : Decidable names} :
     add_global_funs GFuns1 names FVs GFuns2 ->
-    GFun_inv k rho rho' Scope1 (GFuns1 \\ names) σ ->
-    GFun_inv k rho rho' Scope2 GFuns2 σ ->
+    GFun_inv k rho rho' Scope1 (GFuns1 \\ names) ->
+    GFun_inv k rho rho' Scope2 GFuns2 ->
     Scope2 \subset Scope1 ->
-    Disjoint _ Scope1 (image σ names) ->
-    GFun_inv k rho rho' Scope1 GFuns2 σ.
+    Disjoint _ Scope1 names ->
+    GFun_inv k rho rho' Scope1 GFuns2.
   Proof.
     intros Ha Hg1 Hg2 Hsub Hd' x v c Hin1 Hget. inv Ha.
     - destruct Hd. destruct (Dec x); eauto.
       * edestruct Hg2 as (rho1 & B1 & f1 & rho2 & B2 & f2 & Heq1 & Hnin & Hget1 & Hcc); eauto.
         repeat eexists; eauto.
         intros Hc. eapply Hd'. constructor; eauto.
-        eapply In_image. eassumption.
       * inv Hin1; try contradiction.  
         edestruct Hg1 as (rho1 & B1 & f1 & rho2 & B2 & f2 & Heq1 & Hnin & Hget1 & Hcc); eauto.
         constructor; eauto.
@@ -795,12 +765,12 @@ Section Closure_conversion_invariants.
     - eauto.
   Qed.
 
-  Lemma Fun_inv_from_GFun_inv k rho1 rho2 Scope GFuns Funs σ Γ c B :
+  Lemma Fun_inv_from_GFun_inv k rho1 rho2 Scope GFuns Funs Γ c B :
     Funs \subset GFuns ->
     Funs \subset name_in_fundefs B ->
-    GFun_inv k rho1 rho2 Scope (GFuns \\ Scope) σ ->
+    GFun_inv k rho1 rho2 Scope (GFuns \\ Scope) ->
     M.get Γ rho2 = Some (Vconstr c []) ->  
-    Fun_inv k rho1 rho2 Scope Funs σ (extend_fundefs' id B Γ).
+    Fun_inv k rho1 rho2 Scope Funs (extend_fundefs' id B Γ).
   Proof.
     intros Hsub Hsub' Hinv Hget f v' Hnin Hin Hget'.
     edestruct Hinv as
